very wip

Oneshot/lean3-in/main.lean
@@ -1,10 +1,50 @@
--- Insert lean 3 code here.
+-- meta def m := `[skip]
+
+structure finsupp2 (α : Type*) :=
+(to_fun : α → nat)
+(support : list α)
+(mem_support_to_fun : ∀ a, a ∈ support ↔ to_fun a ≠ 0)
+
+inductive hello_world : Type
+| mk : nat → hello_world
+
+def a : _ := @finsupp2.mem_support_to_fun
+
+def blah : Type := Prop
+
+namespace blah
+
+def two_words (x : blah) : ℕ := 1
+
+theorem two_words_eq (x : blah) : two_words x = 1 := rfl
+
+end blah
 
 namespace foo
 
-/-- test -/
+open blah
+
+-- /-- test -/
 @[simp] def foo := 1
 
 theorem foo_eq_one : foo.foo = 1 := rfl
+
+theorem moo (x : blah) : x.two_words = 1 := rfl
+
+theorem moo2 (x : blah) : two_words x = 1 := by rw [two_words_eq]
+
+theorem moo3 (x : blah) : two_words x = 1 := by rw [x.two_words_eq]
+
+theorem moo4 (x : blah) : two_words x = 1 := by refine x.two_words_eq
+
+theorem moo5 (x : blah) : two_words x = 1 := by apply x.two_words_eq
+
+theorem moo6 (x : blah) : two_words x = 1 := by refine two_words_eq _
+
+theorem moo7 (x : blah) : two_words x = 1 := by apply two_words_eq
+
+theorem moo8 (x : blah) : two_words x = 1 := x.two_words_eq
+
+theorem moo9 (x : blah) : two_words x = 1 := two_words_eq _
 
 end foo
